\documentclass[../practica_04.tex]{subfiles}

\begin{document}

    \section*{Definici√≥n}

    $f:\real^2 \rightarrow \real$ es diferenciable en $(a,b) \in \real^2 \Leftrightarrow$

    \begin{enumerate}
        \item $\exists (f_x(a,b) \wedge f_y(a,b))$
        \item $\lim_{(x,y)\to(a,b)} \frac{f(x,y)-f(a,b)-f_x(a,b)(x-a)-f_y(a,b)(y-b)}{\norm*{(x,y)-(a,b)}} = 0 $
    \end{enumerate}

    \section*{Ejericios}

    \begin{enumerate}
        \item 
            \begin{itemize}
                \item $f(x,y) = 1 + x\ln(xy - 5)$
                \item $P = (2,3)$
                \item $f_x(x,y) = \ln(xy-5) + \frac{xy}{xy-5}$
                \item $f_y(x,y) = \frac{x^2}{xy-5}$
                \item $f(2,3) = 1$
                \item $f_x(2,3) = 6$
                \item $f_y(2,3) = 4$
                \item $\lim_{(x,y)\to(2,3)} \frac{1 + x\ln(xy - 5) - 1 - 6(x-2) - 4(y-3)}{\norm*{(x-2,y-3)}} \stackrel{?}{=} 0$
            \end{itemize}

            $\lim_{(x,y)\to(2,3)} \frac{\cancel{1} + x\ln(xy - 5) \cancel{- 1} - 6(x-2) - 4(y-3)}{\norm*{(x-2,y-3)}} =$
            
            $\lim_{(x,y)\to(2,3)} \frac{x\ln(xy - 5) - 6(x-2) - 4(y-3)}{\norm*{(x-2,y-3)}} =$

            $\lim_{(x,y)\to(2,3)} \frac{x\ln(xy - 5) - 2(3(x-2) + 2(y-3))}{\norm*{(x-2,y-3)}} =$

            Pruebo por curvas

            \begin{itemize}
                \item $ y = x + 1$

                    $\lim_{x\to2} \frac{x\ln(x(x+1) - 5) - 6(x-2) - 4((x+1)-3)}{\norm*{(x-2,x-2)}} =$
                \item  No se
            \end{itemize}

        \item 
            \begin{itemize}
                \item $f(x,y) = 
                    \left\{
                        \begin{array}{ll}
                            \frac{x^2y}{x^2+y^2} \qquad si\ (x,y) \neq (0,0)\\
                            0 \qquad si\ (x,y) = (0,0)
                        \end{array}
                    \right.$
                \item $P=(0,0)$
            \end{itemize}

                No es diferenciable en el origen
    \end{enumerate}

\end{document}
