\documentclass[../practica_03.tex]{subfiles}

\begin{document}

    \begin{enumerate}
        \item $f(x,y) = \frac{x^4y^4}{(x^2+y^4)^3}$

            $ \lim_{x \to 0 }  f(x,mx) \equiv $

            $ \lim_{x \to 0 } \frac{x^8m^4}{(x^2+(mx)^4)^3} = $

            $ \lim_{x \to 0 } \frac{x^8m^4}{(x^4+2x^2(mx)^4+(mx)^8)((x^2+(mx)^4)}$

            $ \lim_{x \to 0 } \frac{x^8m^4}{x^6+ 3x^8m^4 + 3x^{10}m^8 + m^{12}x^{12}} = 0$

        \item $f(x,y) = \frac{x^2}{x^2+y^2-x}$

            $ \lim_{x \to 0 }  f(x,mx) \equiv $

            $ \lim_{x \to 0 }  \frac{x^2}{x^2+mx^2-x} = $
            
            $ \lim_{x \to 0 }  \frac{x^{\cancel{2}}}{\cancel{x}(x(1+m)-1)} = 0 $
            
            $ \lim_{x \to 0 }  f(x, x) = $

            $ \lim_{x \to 0 }  \frac{x^2}{x^2\cancel{+x}\cancel{-x}} = 1$

            Si $m=0$ da 1, sino 0 $\Rightarrow \ \nexists L$

    \end{enumerate}

\end{document} 
