\documentclass[../parcial.tex]{subfiles}

\begin{document}

    $ f(1,4) = z(1,4) = 3(1) - 4 + 7 = 6$

    $ f_x(1,4) = z_x(1,4) = 3$

    $ f_y(1,4) = z_y(1,4) = -1$

    $ \left\{
        \begin{array}{ll}
            x(s,t) = \cos(s)t^2 \\
            y(s,y) = (s+2t)^2
        \end{array}
    \right.$

    $ \left\{
        \begin{array}{ll}
            x_s(s,t) = -\sin(s)t^2 \\
            x_t(s,t) = 2\cos(s)t \\
            y_s(s,t) = 2(s+2t)\\
            y_t(s,t) = 4(s+2t)
        \end{array}
    \right.$

    $F(s,t) = f(x(s,t),y(s,t))$

    \begin{enumerate}
        \item $\frac{\partial f}{\partial s} = \frac{\partial f}{\partial x} \cdot \frac{\partial x}{\partial s} + \frac{\partial f}{\partial y} \cdot \frac{\partial y}{\partial s} = $
        
            $f_x(1,4)\cdot x_s(0,-1) + f_y(1,4) \cdot y_s(0,-1) = $

            $3 \cdot 0 + (-1) \cdot 4 = -4$

        \item $\frac{\partial f}{\partial t} = \frac{\partial f}{\partial x} \cdot \frac{\partial t}{\partial s} + \frac{\partial f}{\partial y} \cdot \frac{\partial y}{\partial t}$
        
            $f_x(1,4)\cdot x_t(0,-1) + f_y(1,4) \cdot y_t(0,-1) = $

            $3\cdot (-2) + (-1) \cdot -8 = -6 + 8 = 2 $

    \end{enumerate}

    $ z = \grad F(0,-1)\cdot(s,t+1) + F(0,-1) = $

    \subsection*{$\grad F(0,-1)$ ya lo calculamos antes}

    $ \grad F(s,t) = (-4, 2) $

    $\Rightarrow z = (-4,2)\cdot(s,t+1) + f(1,4)$

    $\Rightarrow z = -4s +2(t+1) + 6$

\end{document} 
