\documentclass[../practica_02.tex]{subfiles}

\begin{document}

    \begin{enumerate}
        \item
            \begin{enumerate}
                \item $x^2 + \frac{y^2}{4} + \frac{z^2}{9} = 1$

                    \begin{itemize}
                        \item
                            \begin{itemize}
                                \item $\stackrel{z=-2}{\Rightarrow} x^2 + \frac{ỵ^2}{9} + \frac{4}{9} = 1$ Una elipse
                                \item $\stackrel{z=-1}{\Rightarrow} x^2 + \frac{ỵ^2}{9} + \frac{1}{9} = 1$ Una elipse
                                \item $\stackrel{z=0}{\Rightarrow} x^2 + \frac{ỵ^2}{9} = 1$ Circulo
                                \item $\stackrel{z=1}{\Rightarrow} x^2 + \frac{ỵ^2}{9} + \frac{1}{9} = 1$ Una elipse
                                \item $\stackrel{z=2}{\Rightarrow} x^2 + \frac{ỵ^2}{9} + \frac{4}{9} = 1$ Una elipse
                            \end{itemize}

                        \item
                            \begin{itemize}
                                \item $\stackrel{y=-2}{\Rightarrow} x^2 + \frac{4}{9} + \frac{z^2}{9} = 1$ Una elipse
                                \item $\stackrel{y=-1}{\Rightarrow} x^2 + \frac{1}{9} + \frac{z^2}{9} = 1$ Una elipse
                                \item $\stackrel{y=0}{\Rightarrow} x^2 + \frac{z^2}{9} = 1$ Circulo
                                \item $\stackrel{y=1}{\Rightarrow} x^2 + \frac{1}{9} + \frac{z^2}{9} = 1$ Una elipse
                                \item $\stackrel{y=2}{\Rightarrow} x^2 + \frac{4}{9} + \frac{z^2}{9} = 1$ Una elipse
                            \end{itemize}

                        \item
                            \begin{itemize}
                                \item $\stackrel{x=-2}{\Rightarrow} 4 + \frac{ỵ^2}{9} + \frac{z^2}{9} = 1$ Circulo
                                \item $\stackrel{x=-1}{\Rightarrow} 1 + \frac{ỵ^2}{9} + \frac{z^2}{9} = 1$ Circulo
                                \item $\stackrel{x=0}{\Rightarrow} \frac{ỵ^2}{9} + \frac{z^2}{9} = 1$ Circulo
                                \item $\stackrel{x=1}{\Rightarrow} 1 + \frac{ỵ^2}{9} + \frac{z^2}{9} = 1$ Circulo
                                \item $\stackrel{x=2}{\Rightarrow} 4 + \frac{ỵ^2}{9} + \frac{z^2}{9} = 1$ Circulo
                            \end{itemize}

                    \end{itemize}

                \item $z = x^2 + y^2$

                    \begin{itemize}
                        \item
                            \begin{itemize}
                                \item $\stackrel{z=0}{\Rightarrow} x^2 + y^2 = 0$ un punto
                                \item $\stackrel{z=1}{\Rightarrow} x^2 + y^2 = 1$ Un circulo con centro en (0,0) y radio 1
                                \item $\stackrel{z=2}{\Rightarrow} x^2 + y^2 = 2$ Un circulo con centro en (0,0) y radio $\sqrt(2)$
                            \end{itemize}

                        \item
                            \begin{itemize}
                                \item $\stackrel{y=-2}{\Rightarrow} x^2 + 4 = z $ Una parabola
                                \item $\stackrel{y=-1}{\Rightarrow} x^2 + 1 = z $ Una parabola
                                \item $\stackrel{y=0}{\Rightarrow} x^2 +  0 = z $ Una parabola
                                \item $\stackrel{y=1}{\Rightarrow} x^2 +  1 = z $ Una parabola
                                \item $\stackrel{y=2}{\Rightarrow} x^2 +  4 = z $ Una parabola
                            \end{itemize}

                        \item
                            \begin{itemize}
                                \item $\stackrel{x=-2}{\Rightarrow} 4 + y^2 = z $ Una parabola
                                \item $\stackrel{x=-1}{\Rightarrow} 1 + y^2 = z $ Una parabola
                                \item $\stackrel{x=0}{\Rightarrow}  0 + y^2  = z $ Una parabola
                                \item $\stackrel{x=1}{\Rightarrow}  1 + y^2  = z $ Una parabola
                                \item $\stackrel{x=2}{\Rightarrow}  4 + y^2  = z $ Una parabola
                            \end{itemize}

                    \end{itemize}

                \item $x = y^2 + 4z^2$

                    \begin{itemize}
                        \item
                            \begin{itemize}
                                \item $\stackrel{z=-2}{\Rightarrow} x = y^2 + 16 $ Una parabola
                                \item $\stackrel{z=-1}{\Rightarrow} x = y^2 + 4 $ Una parabola
                                \item $\stackrel{z=0}{\Rightarrow} x = y^2 +  $ Una parabola
                                \item $\stackrel{z=1}{\Rightarrow} x = y^2 + 4 $ Una parabola
                                \item $\stackrel{z=2}{\Rightarrow} x = y^2 + 16 $ Una parabola
                            \end{itemize}

                        \item
                            \begin{itemize}
                                \item $\stackrel{y=-2}{\Rightarrow} x = 4 + 4z^2 $ Una parabola
                                \item $\stackrel{y=-1}{\Rightarrow} x = 1 + 4z^2 $ Una parabola
                                \item $\stackrel{y=0}{\Rightarrow} x = 0 + 4z^2 $ Una parabola
                                \item $\stackrel{y=1}{\Rightarrow} x = 1 + 4z^2 $ Una parabola
                                \item $\stackrel{y=2}{\Rightarrow} x = 4 + 4z^2 $ Una parabola
                            \end{itemize}

                        \item
                            \begin{itemize}
                                \item $\stackrel{x=0}{\Rightarrow}  x = y^2 + 4z^2 $ Un punto
                                \item $\stackrel{x=1}{\Rightarrow}  1 = y^2 + 4z^2 $ Una elipse
                                \item $\stackrel{x=2}{\Rightarrow}  2 = y^2 + 4z^2 $ Una elipse
                            \end{itemize}

                    \end{itemize}

                \item $z^2 = x^2 + y^2$

                    \begin{itemize}
                        \item
                            \begin{itemize}
                                \item $\stackrel{z=-2}{\Rightarrow}  4 = x^2 + y^2 $ Un circulo con centro en (0,0) y radio $\sqrt(2)$
                                \item $\stackrel{z=-1}{\Rightarrow}  1 = x^2 + y^2 $ Un circulo con centro en (0,0) y radio 1
                                \item $\stackrel{z=0}{\Rightarrow}   0 = x^2 + y^2 $ Un punto
                                \item $\stackrel{z=1}{\Rightarrow}   1 = x^2 + y^2 $ Un circulo con centro en (0,0) y radio 1
                                \item $\stackrel{z=2}{\Rightarrow}   4 = x^2 + y^2 $ Un circulo con centro en (0,0) y radio $\sqrt(2)$
                            \end{itemize}

                        \item
                            \begin{itemize}
                                \item $\stackrel{y=-2}{\Rightarrow} z^2 - x^2 = 4 $ Hiperbola
                                \item $\stackrel{y=-1}{\Rightarrow} z^2 - x^2 = 1 $ Hiperbola
                                \item $\stackrel{y=0}{\Rightarrow}  z^2 - x^2 = 0 $ Una X
                                \item $\stackrel{y=1}{\Rightarrow}  z^2 - x^2 = 1 $ Hiperbola
                                \item $\stackrel{y=2}{\Rightarrow}  z^2 - x^2 = 4 $ Hiperbola
                            \end{itemize}

                        \item
                            \begin{itemize}
                                \item $\stackrel{x=-2}{\Rightarrow} z^2 - y^2 = 4 $ Hiperbola
                                \item $\stackrel{x=-1}{\Rightarrow} z^2 - y^2 = 1 $ Hiperbola
                                \item $\stackrel{x=0}{\Rightarrow}  z^2 - y^2 = 0 $ Una x
                                \item $\stackrel{x=1}{\Rightarrow}  z^2 - y^2 = 1 $ Hiperbola
                                \item $\stackrel{x=2}{\Rightarrow}  z^2 - y^2 = 4 $ Hiperbola
                            \end{itemize}

                    \end{itemize}

                \item $x^2 = y^2 + 4z^2$

                    \begin{itemize}
                        \item
                            \begin{itemize}
                                \item $\stackrel{z=-2}{\Rightarrow}  x^2 = y^2 + 16 $ Hiperbola
                                \item $\stackrel{z=-1}{\Rightarrow}  x^2 = y^2 + 4  $ Hiperbola
                                \item $\stackrel{z=0}{\Rightarrow}   x^2 = y^2      $ Un punto
                                \item $\stackrel{z=1}{\Rightarrow}   x^2 = y^2 + 4  $ Hiperbola
                                \item $\stackrel{z=2}{\Rightarrow}   x^2 = y^2 + 16 $ Hiperbola
                            \end{itemize}

                        \item
                            \begin{itemize}
                                \item $\stackrel{y=-2}{\Rightarrow} x^2 = 4 + 4z^2 $ Hiperbola
                                \item $\stackrel{y=-1}{\Rightarrow} x^2 = 1 + 4z^2 $ Hiperbola
                                \item $\stackrel{y=0}{\Rightarrow}  x^2 = 4z^2     $ Una X
                                \item $\stackrel{y=1}{\Rightarrow}  x^2 = 1 + 4z^2 $ Hiperbola
                                \item $\stackrel{y=2}{\Rightarrow}  x^2 = 4 + 4z^2 $ Hiperbola
                            \end{itemize}

                        \item
                            \begin{itemize}
                                \item $\stackrel{x=-2}{\Rightarrow} 4 = y^2 + 4z^2 $ Un elipse
                                \item $\stackrel{x=-1}{\Rightarrow} 1 = y^2 + 4z^2 $ Un elipse
                                \item $\stackrel{x=0}{\Rightarrow}  0 = y^2 + 4z^2 $ Un punto
                                \item $\stackrel{x=1}{\Rightarrow}  1 = y^2 + 4z^2 $ Un elipse
                                \item $\stackrel{x=2}{\Rightarrow}  4 = y^2 + 4z^2 $ Un elipse
                            \end{itemize}

                    \end{itemize}

                \item $z = x^2 - y^2$

                    \begin{itemize}
                        \item
                            \begin{itemize}
                                \item $\stackrel{z=-2}{\Rightarrow} -2 = x^2 - y^2 $ Hiperbola
                                \item $\stackrel{z=-1}{\Rightarrow} -1 = x^2 - y^2 $ Hiperbola
                                \item $\stackrel{z=0}{\Rightarrow} y^2 = x^2       $ Ejes de $45^\circ$
                                \item $\stackrel{z=1}{\Rightarrow}   1 = x^2 - y^2 $ Hiperbola
                                \item $\stackrel{z=2}{\Rightarrow}   2 = x^2 - y^2 $ Hiperbola
                            \end{itemize}

                        $ $

                        \item
                            \begin{itemize}
                                \item $\stackrel{y=-2}{\Rightarrow} z = x^2 - 4 $ Parabola
                                \item $\stackrel{y=-1}{\Rightarrow} z = x^2 - 1 $ Parabola
                                \item $\stackrel{y=0}{\Rightarrow}  z = x^2 - 0 $ Parabola
                                \item $\stackrel{y=1}{\Rightarrow}  z = x^2 - 1 $ Parabola
                                \item $\stackrel{y=2}{\Rightarrow}  z = x^2 - 4 $ Parabola
                            \end{itemize}

                            $ $

                        \item
                            \begin{itemize}
                                \item $\stackrel{x=-2}{\Rightarrow} z = 4 - y^2 $ Parabola
                                \item $\stackrel{x=-1}{\Rightarrow} z = 1 - y^2 $ Parabola
                                \item $\stackrel{x=0}{\Rightarrow}  z = 0 - y^2 $ Parabola
                                \item $\stackrel{x=1}{\Rightarrow}  z = 1 - y^2 $ Parabola
                                \item $\stackrel{x=2}{\Rightarrow}  z = 4 - y^2 $ Parabola
                            \end{itemize}

                            $ $
                    \end{itemize}

                \item $x^2 + y^2 - z^2 = 1$

                    \begin{itemize}
                        \item
                            \begin{itemize}
                                \item $\stackrel{z=-2}{\Rightarrow} x^2 + y^2 - 4 = 1 $ Circulo
                                \item $\stackrel{z=-1}{\Rightarrow} x^2 + y^2 - 1 = 1 $ Circulo
                                \item $\stackrel{z=0}{\Rightarrow}  x^2 + y^2 - 0 = 1 $ Circulo
                                \item $\stackrel{z=1}{\Rightarrow}  x^2 + y^2 - 1 = 1 $ Circulo
                                \item $\stackrel{z=2}{\Rightarrow}  x^2 + y^2 - 4 = 1 $ Circulo
                            \end{itemize}

                        $ $

                        \item
                            \begin{itemize}
                                \item $\stackrel{y=-2}{\Rightarrow} x^2 + 4 - z^2 = 1 $ Hiperbola
                                \item $\stackrel{y=-1}{\Rightarrow} x^2 + 1 - z^2 = 1 $ Hiperbola
                                \item $\stackrel{y=0}{\Rightarrow}  x^2 + 0 - z^2 = 1 $ Hiperbola
                                \item $\stackrel{y=1}{\Rightarrow}  x^2 + 1 - z^2 = 1 $ Hiperbola
                                \item $\stackrel{y=2}{\Rightarrow}  x^2 + 4 - z^2 = 1 $ Hiperbola
                            \end{itemize}

                            $ $

                        \item
                            \begin{itemize}
                                \item $\stackrel{x=-2}{\Rightarrow} 4 + y^2 - z^2 = 1 $ Hiperbola
                                \item $\stackrel{x=-1}{\Rightarrow} 1 + y^2 - z^2 = 1 $ Hiperbola
                                \item $\stackrel{x=0}{\Rightarrow}  0 + y^2 - z^2 = 1 $ Hiperbola
                                \item $\stackrel{x=1}{\Rightarrow}  1 + y^2 - z^2 = 1 $ Hiperbola
                                \item $\stackrel{x=2}{\Rightarrow}  4 + y^2 - z^2 = 1 $ Hiperbola
                            \end{itemize}

                            $ $
                    \end{itemize}

                \item $- x^2 - y^2 + z^2 = 1$

                    \begin{itemize}
                        \item
                            \begin{itemize}
                                \item $\stackrel{z=-2}{\Rightarrow} - x^2 - y^2 + 4 = 1 $ Circulo
                                \item $\stackrel{z=-1}{\Rightarrow} - x^2 - y^2 + 2 = 1 $ Circulo
                                \item $\stackrel{z=0}{\Rightarrow}  - x^2 - y^2 + 1 = 1 $ Circulo
                                \item $\stackrel{z=1}{\Rightarrow}  - x^2 - y^2 + 2 = 1 $ Circulo
                                \item $\stackrel{z=2}{\Rightarrow}  - x^2 - y^2 + 4 = 1 $ Circulo
                            \end{itemize}

                        $ $

                        \item
                            \begin{itemize}
                                \item $\stackrel{y=-2}{\Rightarrow} - x^2 - 4 + z^2 = 1 $ Hiperbola
                                \item $\stackrel{y=-1}{\Rightarrow} - x^2 - 2 + z^2 = 1 $ Hiperbola
                                \item $\stackrel{y=0}{\Rightarrow}  - x^2 - 1 + z^2 = 1 $ Hiperbola
                                \item $\stackrel{y=1}{\Rightarrow}  - x^2 - 2 + z^2 = 1 $ Hiperbola
                                \item $\stackrel{y=2}{\Rightarrow}  - x^2 - 4 + z^2 = 1 $ Hiperbola
                            \end{itemize}

                            $ $

                        \item
                            \begin{itemize}
                                \item $\stackrel{x=-2}{\Rightarrow} - 4 - y^2 + z^2 = 1 $ Hiperbola
                                \item $\stackrel{x=-1}{\Rightarrow} - 2 - y^2 + z^2 = 1 $ Hiperbola
                                \item $\stackrel{x=0}{\Rightarrow}  - 1 - y^2 + z^2 = 1 $ Hiperbola
                                \item $\stackrel{x=1}{\Rightarrow}  - 2 - y^2 + z^2 = 1 $ Hiperbola
                                \item $\stackrel{x=2}{\Rightarrow}  - 4 - y^2 + z^2 = 1 $ Hiperbola
                            \end{itemize}

                            $ $
                    \end{itemize}

                \item $4x^2 + 9y^2 + z = 0$

                    \begin{itemize}
                        \item
                            \begin{itemize}
                                \item $\stackrel{z=-2}{\Rightarrow} 4x^2 + 9y^2 +(-2) = 0 $ Elipse
                                \item $\stackrel{z=-1}{\Rightarrow} 4x^2 + 9y^2 +(-1) = 0 $ Elipse
                                \item $\stackrel{z=0}{\Rightarrow}  4x^2 + 9y^2       = 0 $ Elipse
                                \item $\stackrel{z=1}{\Rightarrow}  4x^2 + 9y^2 + 1   = 0 $ Elipse
                                \item $\stackrel{z=2}{\Rightarrow}  4x^2 + 9y^2 + 2   = 0 $ Elipse
                            \end{itemize}

                        $ $

                        \item
                            \begin{itemize}
                                \item $\stackrel{y=-2}{\Rightarrow} 4x^2 + 18 + z = 0 $ Parabola
                                \item $\stackrel{y=-1}{\Rightarrow} 4x^2 + 9  + z = 0 $ Parabola
                                \item $\stackrel{y=0}{\Rightarrow}  4x^2 +    + z = 0 $ Parabola
                                \item $\stackrel{y=1}{\Rightarrow}  4x^2 + 9  + z = 0 $ Parabola
                                \item $\stackrel{y=2}{\Rightarrow}  4x^2 + 18 + z = 0 $ Parabola
                            \end{itemize}

                            $ $

                        \item
                            \begin{itemize}
                                \item $\stackrel{x=-2}{\Rightarrow} 16 + 9y^2 + z = 0 $ Parabola
                                \item $\stackrel{x=-1}{\Rightarrow}  4 + 9y^2 + z = 0 $ Parabola
                                \item $\stackrel{x=0}{\Rightarrow}       9y^2 + z = 0 $ Parabola
                                \item $\stackrel{x=1}{\Rightarrow}   4 + 9y^2 + z = 0 $ Parabola
                                \item $\stackrel{x=2}{\Rightarrow}  16 + 9y^2 + z = 0 $ Parabola
                            \end{itemize}

                            $ $
                    \end{itemize}

            \end{enumerate}
        \item
            \begin{enumerate}
                \item 
            \end{enumerate}
    \end{enumerate}

\end{document}