\documentclass[../parcial.tex]{subfiles}

\begin{document}

    \begin{enumerate}
        \item $ \lim_{(x,y) \to (0,0)} f(x,y) $

            $f(x,y) = \frac{(x-1)^2x^2y^2}{(x^2+y^2)^{\frac{3}{2}}}$

            \subsection*{Pruebo por curvas}

            \begin{itemize}
                \item iterado $x = 0$

                    $\lim_{y\to0} f(0,y) = \frac{0}{(y^2)^{\frac{3}{2}}} = 0$

                \item iterado $y = 0$

                    $\lim_{x\to0} f(x,0) = \frac{0}{(x^2)^{\frac{3}{2}}} = 0$

            \end{itemize}

            si $\exists L: \lim_{(x,y) \to (0,0)} f(x,y) \Rightarrow L = 0 $

            \subsection*{Intento demostrar por sandwich}
        
            $ \exists g(x,y): \lim{(x,y)\to(0,0)} g(x,y) = 0 \wedge 0 \leq \abs*{f(x,y)} \leq \abs*{g(x,y)} $

            $ \abs*{f(x,y)} = \abs*{\frac{(x-1)^2x^2y^2}{(x^2+y^2)^{\frac{3}{2}}}} = $

            $ \frac{(x-1)^2x^2y^2}{(x^2+y^2)^{\frac{3}{2}}} =  $

            $ \frac{(x-1)^2x^2y^2}{(x^2+y^2)^{\frac{3}{2}}} \cdot \frac{(x^2+y^2)^{\frac{2}{3}}}{(x^2+y^2)^{\frac{2}{3}}} = $

            $ \frac{(x-1)^2x^2y^2(x^2+y^2)^{\frac{2}{3}}}{x^2+y^2} = $

            $ \frac{y^2}{x^2+y^2} \cdot (x-1)^2x^2(x^2+y^2)^{\frac{2}{3}} $

            \qquad $ x^2 \geq 0 \Rightarrow x^2 + y^2 \geq y^2 \Rightarrow 1 \geq \frac{y^2}{x^2 + y^2} : \star $

            $ \frac{y^2}{x^2+y^2} \cdot (x-1)^2x^2(x^2+y^2)^{\frac{2}{3}} \stackrel{\star}{\leq}$

            $ 1 \cdot (x-1)^2x^2(x^2+y^2)^{\frac{2}{3}} =  $

            $ (x-1)^2x^2(x^2+y^2)^{\frac{2}{3}} \stackrel{(x,y) \to (0,0)}{\to} 0 $

            $ \Rightarrow g(x,y) = (x-1)^2x^2(x^2+y^2)^{\frac{2}{3}} $

            $ 0 \leq \abs*{f(x,y)} \leq \abs*{g(x,y)} $

            $ \Rightarrow \exists L \wedge L = 0 \qquad \square$

        \item $ \lim_{(x,y) \to (0,0)} f(x,y) $
        
            $f(x,y)$
        
            \subsection*{Pruebo por curvas}

            \begin{itemize}
                \item iterado $ x = 0$

                    $\lim_{y\to0} f(0,y)$

                \item iterado $ y = 0$

                    $\lim_{x\to0} f(x,0)$

                \item rectas $ y = mx$
                
                    $\lim_{x\to0} f(x,mx)$

                \item curvas $ y = x^2$

                    $\lim_{x\to0} f(x,x^2)$

            \end{itemize}

            \subsection*{Intento demostrar por sandwich}
        
            $ \exists g(x,y): \lim{(x,y)\to(0,0)} g(x,y) = 0 \wedge 0 \leq \abs*{f(x,y)} \leq \abs*{g(x,y)} $
        
            \subsection*{Pruebo por definiciÃ³n}

            $ \exists \epsilon,\delta(\epsilon) > 0 : \norm*{(x,y) - (0,0)} < \delta \Rightarrow \abs*{f(x,y)} < \epsilon $

    \end{enumerate}

\end{document} 
