\documentclass[../practica_04.tex]{subfiles}

\begin{document}

    \begin{enumerate}
        \item $f(x,y,z) = \sqrt{\abs*{xyz}}$
            No existen las derivadas parciales en el origen

        \item $f(x,y) = 
            \left\{
                \begin{array}{ll}
                    \frac{x^4-y^4}{x^2+y^2} \qquad si\ (x,y) \neq (0,0)\\
                    0 \qquad si\ (x,y) = (0,0)
                \end{array}
            \right.$

            $f_x(0,0) = \lim_{x\to} \frac{f(h,0)-f(0,0)}{h} = $

            $\lim_{h\to0} \frac{\frac{h^4}{h^2}}{h} = $

            $\lim_{h\to0} \frac{h\cancel{^4}}{\cancel{h^3}} = 0 $

            $f_y(0,0) = \lim_{h\to0} \frac{f(0,h)-f(0,0)}{h} = $

            $\lim_{h\to0} \frac{\frac{-h^4}{h^2}}{h} = $

            $\lim_{h\to0} \frac{-h\cancel{^4}}{\cancel{h^3}} = 0 $

            $\lim_{(x,y)\to(0,0)} \frac{\frac{x^4-y^4}{x^2+y^2}}{\norm*{x^2+y^2}} \stackrel{?}{=} 0 $

            $\lim_{(x,y)\to(0,0)} \frac{\frac{x^4-y^4}{\norm*{x^2+y^2}^2}}{\norm*{x^2+y^2}} = $

            $\lim_{(x,y)\to(0,0)} \frac{x^4-y^4}{\norm*{x^2+y^2}^3}  $

            $\lim_{(x,y)\to(0,0)} \frac{\abs*{x^4-y^4}}{\norm*{x^2+y^2}^3} \stackrel{DesTrian}{\leq} $

            $\lim_{(x,y)\to(0,0)} \frac{x^4+y^4}{\norm*{x^2+y^2}^3} \leq $

            $\lim_{(x,y)\to(0,0)} \frac{2\norm*{x^2+y^2}\cancel{^4}}{\cancel{\norm*{x^2+y^2}^3}} \leq $

            $ 2 \lambda < \epsilon \Rightarrow \lambda \leq \frac{\epsilon}{2}$

            $\Pi: z = 0$

        \item $f(x,y) = 
            \left\{
                \begin{array}{ll}
                    \frac{x^2}{x^2+y^2}\cdot \sin(\frac{1}{\sqrt{x^2+y^2}}) \qquad si\ (x,y) \neq (0,0)\\
                    0 \qquad si\ (x,y) = (0,0)
                \end{array}
            \right.$

            $f_x(0,0) = \lim_{h\to0} \frac{f(h,0)-f(0,0)}{h} = $

                $\lim_{h\to0} \frac{\cancel{\frac{h^2}{h^2}}\cdot \sin(\frac{1}{\sqrt{h^2}})}{h} = $

                $\lim_{h\to0} \frac{\sin(\frac{1}{\sqrt{h^2}})}{h} = $

                $\lim_{h\to0} \frac{\sin(\frac{1}{\sqrt{h^2}})}{h} = \nexists $

                $\Rightarrow$ No es diferenciable en el origen

    \end{enumerate}

\end{document}
