\documentclass[../parcial.tex]{subfiles}

\begin{document}

    $f(x,y) = \cos(y)e^{2x}$

    \begin{itemize}
        \item $f_x(x,y) = 2\cos(y)e^{2x}$
        \item $f_y(x,y) = -\sin(y)e^{2x}$
        \item $f_xx(x,y) = 4\cos(y)e^{2x}$
        \item $f_xy(x,y) = -2\sin(y)e^{2x}$
        \item $f_yy(x,y) = -\cos(y)e^{2x}$
    \end{itemize}

    \begin{itemize}
        \item $f(0,0) = 1$
        \item $f_x(0,0) = 2$
        \item $f_y(0,0) = 0$
        \item $f_xx(0,0) = 4$
        \item $f_xy(0,0) = 0$
        \item $f_yy(0,0) = -1$
    \end{itemize}

    $P_2(x,y) = 1 + 2x + 2x^2 - \frac{y^2}{2} + R_2(x,y)$

    $\Rightarrow \cos(y)e^{2x} - (1 + 2x + 2x^2 - \frac{y^2}{2}) \equiv $

    $ \cancel{1 + 2x + 2x^2 - \frac{y^2}{2}} + R_2(x,y) - \cancel{(1 + 2x + 2x^2 - \frac{y^2}{2})} = $

    $ R_2(x,y) \Rightarrow$

    $\lim_{(x,y) \to (0,0)} \frac{\cos(y)e^{2x} - (1 + 2x + 2x^2 - \frac{y^2}{2})}{x^2+y^2} = \lim_{(x,y) \to (0,0)} \frac{R_2(x,y)}{x^2+y^2} = 0$

\end{document}
