\documentclass[../practica_08.tex]{subfiles}

\begin{document}

    \begin{enumerate}
        \item $\int_{-2}^{2} (\int_0^{y^2} 1+x^2y^2 dd ) dy = $
        
            \begin{itemize}
                \item $\int_0^{y^2} 1+x^2y^2 dy = $
                
                    $\left. x+\frac{x^3y^2}{3} \right |_0^{y^2} = $

                    $  y^2 + \frac{y^5}{3} $

                \item $\int_{-2}^2 y^2 + \frac{y^5}{3} dy = $
                
                    $ \left. \frac{y^3}{3} + \frac{y^6}{18} \right |_{-2}^2 = $

                    $ \frac{2^3}{3} + \frac{2^6}{18} + \frac{2^3}{3} - \frac{2^6}{18} = $

                    $ \frac{16}{3} $

            \end{itemize}

        \item $ z = 6 -3x -2y  $

            \begin{itemize}
                \item $\int_0^2 (\int_0^{3-\frac{3}{2}x} 6 -3x -2y dy) dx$
                
                    \begin{itemize}
                        \item $\int_0^{3-\frac{3}{2}x} 6 -3x -2y dy = $
                        
                            $ \left. 6y-3xy-y^2 \right |_0^{3-\frac{3}{2}x} = $

                            $ 6(3-\frac{3}{2}x)-3x(3-\frac{3}{2}x)-(3-\frac{3}{2}x)^2 = $

                            $ 18 \cancel{- \frac{18}{2}x} - 9x + \frac{9}{2}x^2 - \frac{9}{4}x^2 \cancel{+ \frac{18}{2}x} - 9 = $

                            $ 9 - 9x + \frac{9}{4}x^2 $

                            $ 9 \cdot(1 - x + \frac{1}{4}x^2) $

                        \item $9 \cdot \int_0^2 1 - x + \frac{1}{4}x^2 dx = $
                        
                            $9 \cdot \left. x - \frac{x^2}{2} + \frac{1}{12}x^3 \right |_0^2 = $

                            $ 9(2 - 2 + \frac{4}{3}) = $

                            $ 12 $

                    \end{itemize}

            \end{itemize}
        
        \item $ \int_0^1 (\int_0^{\sqrt(1-x^2)} y dy) dx$
        
            \begin{itemize}
                \item $\int_0^{\sqrt(1-x^2)} y dy$
                
                    $\left. \frac{y^2}{2} \right |_0^{\sqrt(1-x^2)}$

                    $ \frac{1-x^2}{2} $

                \item $ \frac{1}{2}  \int_0^1 1-x^2 dx = $
                
                    $\frac{1}{2} \left. x - \frac{x^3}{3} \right |_0^1 = $

                    $ \frac{1}{2} (1- \frac{1}{3}) =  $

                    $ \frac{2}{3} $

            \end{itemize}

    \end{enumerate}

\end{document}
