\documentclass[../practica_06.tex]{subfiles}

\begin{document}

    \begin{enumerate}
        \item $f(x,y) = x^2 + xy + y^2 + y$
        
            \begin{itemize}
                \item $f_x(x,y) = 2x + y $

                    $= 0 \Leftrightarrow y = -2x$

                \item $f_y(x,y) = x + 2y + 1 $

                    $= 0 \Leftrightarrow x = -2y -1$

            \end{itemize}

            $\Leftrightarrow x = \frac{1}{3} \wedge y = -\frac{2}{3}$

            $H_f(\frac{1}{3}, -\frac{2}{3}) = \begin{vmatrix}
                2 & 1 \\
                1 & 2
            \end{vmatrix} \Rightarrow det(H_f(\frac{1}{3}, -\frac{2}{3})) = 2$

            $(\frac{1}{3}, -\frac{2}{3})$ es m√≠nimo local de f

        \item $f(x,y) = (x-y)(1-xy) = x - yx^2 - y + xy^2$
        
            \begin{itemize}
                \item $f_x(x,y) = 1 - 2xy + y^2 $
                
                    $ = 0 \Leftrightarrow 0 = 1 + y(-2x + y) $

                    $\Leftrightarrow -1 = y(-2x + y) \Leftrightarrow (x,y) \in \{(1,1),(-1,-1)\}$

                \item $f_y(x,y) = -1 - x^2 + 2xy $
                
                    $ = 0 \Leftrightarrow 0 = -1 + x(-x + 2y)$

            \end{itemize}

            $H_f(x,y) = \begin{vmatrix}
                -2y & -2x + 2y \\
                -2x + 2y & 2x
            \end{vmatrix}$
        
            Ptos criticos \begin{itemize}
                \item $(-1,-1)$
                
                    $H_f(-1,-1) = -4 \Rightarrow$ es punto silla 
                    
                \item $(1,1)$

                    $H_f(1,1) = -4 \Rightarrow$ es punto silla 
            \end{itemize}

        \item $f(x,y) = y^3 + 3x^2y - 6x^2 - 6y^2 + 2$
        
            \begin{itemize}
                \item $f_x(x,y) = 6xy - 12x$
                
                    $ 6x(y-2) = 0 \Leftrightarrow x = 0 \vee y = 2$

                \item $f_y(x,y) = 3y^2 + 3x^2 - 12y$

                    $(-2,2),(2,2),(0,0),(0,4)$

            \end{itemize}

            $H_f(x,y) = \begin{vmatrix}
                6y - 12 & 6x \\
                6x & 6y - 12
            \end{vmatrix}$

            Ptos criticos\begin{itemize}
                \item $(0,0)$
                
                    $H_f(0,0) = -24$ pto silla

                \item $(0,2)$
                
                    $H_f(0,2) = 0 - 0$ maximo 

                \item $(2,2)$
                
                    $H_f(2,2) = 0 - 12^2$ pto silla

                \item $(-2,2)$
                
                    $H_f(-2,2) = 24^2 - 12^2$ maximo

                \item $(0,4)$
                

                    $H_f(0,4) = (4\cdot 12)^2 - 0 $ minimo

            \end{itemize}

        \item $f(x,y) = xy + \frac{1}{x} + \frac{1}{y}$
        
            \begin{itemize}
                \item $f_x(x,y) = y + \frac{-1}{x^2}$
                \item $f_y(x,y) = x + \frac{-1}{y^2}$
            \end{itemize}

            $H_f(x,y) = \begin{vmatrix}
                \frac{2}{x^3} & 1 \\
                1 & \frac{2}{y^3}
            \end{vmatrix}$

            Ptos criticos\begin{itemize}
                \item $(1,-1)$
                
                    $H_f(1,-1) = -4 - 1$ pto silla

                \item $(1,1)$
                
                    $H_f(1,1) = 4 - 1$ minimo
                    
                \item $(-1,1)$
                
                    $H_f(-1,1) = -4 - 1$ pto silla
                \end{itemize}
 
        \item $f(x,y) = y\cos(x)$
        
            \begin{itemize}
                \item $f_x(x,y) = -y\sin(x)$
                \item $f_y(x,y) = \cos(x)$
            \end{itemize}

            $H_f(x,y) = \begin{vmatrix}
                -y\cos(x) && \sin(x)
                -\sin(x) && 1
            \end{vmatrix}$

            Ptos criticos \begin{itemize}
                \item $(0,0)$
                
                    $H_f(0,0) = 0 - 0$ pto silla

                \item $(\frac{\pi}{2},0)$
                
                    $H_f(\frac{\pi}{2},0) = 0 + 1$ pto silla

            \end{itemize}

        \item $f(x,y) = e^y(y^2-x^2) = e^yy^2 - e^yx^2$
        
            \begin{itemize}
                \item $f_x(x,y) = -2xe^y$
                
                    $x = 0$

                \item $f_y(x,y) = e^y(y^2 + 2y) - e^yx^2$
                
                    $ y = 0 \vee y = -2 $

            \end{itemize}

            $H_f(x,y) = \begin{vmatrix}
                -2e^y && -2xe^y\\
                -2xe^y &&  e^y(-x^2 + y^2 + 4y + 2)
            \end{vmatrix}$

            ptos criticos \begin{itemize}
                \item $(0,0)$
                
                    $H_f(0,0) = -2(2) - 0 $ pto silla 
                
                \item $(0,-2)$
                
                    $H_f(0,0) = -4e^{-2} $ pto silla

            \end{itemize}

    \end{enumerate}

\end{document}
