\documentclass[../practica_03.tex]{subfiles}

\begin{document}

    \begin{enumerate}
        \item $\lim_{(x,y)\to(7,2)} x^2+y^2-xy$

            $7^2+2^4-(7\cdot 2) = 39$

        \item $\lim_{(x,y)\to(0,1)} xe^{xy}$

            $0\cdot 1 = 0$

        \item $\lim_{(x,y)\to(2,1)} \frac{4-xy}{x^2+3y^2}$

            $\frac{4-2}{4+3(1)} = \frac{2}{7}$

        \item $\lim_{(x,y)\to(0,0)} = \frac{x-y}{x+y}$
        
            $\lim_{x\to0} f(x,0) = 1 $

            $\lim_{y\to0} f(0,y) = -1 $

            $\Rightarrow Por\ curvas \nexists L$

        \item $\lim_{(x,y)\to(0,0)} = \frac{x^4-4y^2}{x^2+2y^2}$

            $\lim_{x\to0} f(x,0) = 0 $

            $\lim_{y\to0} f(0,y) = -2 $

            $\Rightarrow Por\ curvas \nexists L$

        \item $\lim_{(x,y)\to(0,0)} = \frac{xy}{x^2+y^2}$

            $\lim_{x\to0} f(x,0) = 0 $

            $\lim_{y\to0} f(0,y) = 0 $

            $\lim_{y\to0} f(x,x) = \frac{1}{2} $

            $\Rightarrow Por\ curvas \nexists L$

        \item $\lim_{(x,y)\to(1,0)} = \frac{xy-y}{(x-1)^2+y^2}$

            $\lim_{x\to1} f(x,0) = 0 $

            $\lim_{y\to0} f(0,y) = 0 $

            $\lim_{x\to1} f(x,x) = \frac{x(x-1)}{(x-1)^2 + x^2} = 0 $

            $\lim_{x\to1} f(x,(x-1)) = \frac{(x-1)^2}{2(x-1)^2} = \frac{1}{2} $

            $\Rightarrow Por\ curvas \nexists L$

        \item $\lim_{(x,y)\to(0,0)} = \frac{xy}{\sqrt{x^2+y^2}}$

            $\lim_{x\to0} f(x,0) = 0 $

            $\lim_{y\to0} f(0,y) = 0 $

            Sospecho que $L=0$, lo pruebo por definición

            $\norm*{(x,y)} < \delta \Rightarrow \abs*{\frac{xy}{\sqrt{x^2+y^2}}} < \epsilon $

            \begin{itemize}
                \item $\abs*{x} \leq \norm*{(x,y)} < \delta$
                \item $\abs*{y} \leq \norm*{(x,y)} < \delta$
            \end{itemize}

            $\abs*{\frac{xy}{\sqrt{x^2+y^2}}} = $

            $\frac{\abs*{y}\abs*{y}}{\sqrt{x^2+y^2}} = $

            $\frac{\abs*{y}\abs*{y}}{\sqrt{x^2+y^2}} = $

            $\frac{\abs*{y}\abs*{y}}{\norm*{(x,y)}} \leq $

            $\frac{\norm*{(x,y)}\norm*{(x,y)}}{\norm*{(x,y)}} = $
            
            $\norm*{(x,y)} \leq \delta \Rightarrow \delta = \epsilon \blacksquare$

        \item $\lim_{(x,y)\to(0,0)} = \frac{x^4-y^4}{x^2+y^2}$

            $\frac{x^4-y^4}{x^2+y^2} = $

            $\frac{(x^2-y^2)(x^2+y^2)}{x^2+y^2} = $

            $x^2+y^2$

            $ (x,y) \to (0,0) \Rightarrow x^2+y^2 \to 0 \qquad \blacksquare$

        \item $\lim_{(x,y)\to(0,0)} = \frac{y^2\sin^2(x)}{x^4+2y^4}$

            $\lim_{x\to0} f(x,0) = 0 $

            $\lim_{y\to0} f(0,y) = 0 $

            $\lim_{x\to0} f(x,x) = \lim_{x\to0} \frac{x^2\sin^2(x)}{x^4+2x^4} = $
            
            $\lim_{x\to0} \frac{x^2\sin^2(x)}{3x^4} = $

            $\lim_{x\to0} \frac{\cancel{x^2}}{3\cancel{x^2}} \cdot \stackrel{\to 1}{\frac{\sin(x)}{x}} \cdot \stackrel{\to 1}{\frac{\sin(x)}{x}} = \frac{1}{3} $

            $\Rightarrow \nexists L$

        \item $\lim_{(x,y)\to(0,3)} \frac{x^2(y-3)^2e^x}{x^2+(y-3)^2}$

            \begin{itemize}

                \item $\lim_{x\to0} f(x,0) = \lim_{x\to0} \frac{x^2(-3)^2e^x}{x^2+(-3)^2} = 0 $

                \item $\lim_{y\to3} f(0,y) = \lim_{y\to3} \frac{0}{(y-3)^2} = 0$

                \item $\lim_{y\to3} f(y-3,y) = $
                    $\lim_{y\to3} \frac{\cancel{(y-3)^2}(y-3)^2e^{y-3}}{2\cancel{(y-3)^2}} = $

                    $\lim_{y\to3} \frac{\stackrel{\to 0}{(y-3)^2}\stackrel{\to 1}{e^{y-3}}}{2} = 0$
            \end{itemize}

            Sospecho que $L = 0$ pruebo por definición

            $\norm*{(x,y-3)} < \delta \Rightarrow \abs*{\frac{x^2(y-3)^2e^x}{x^2+(y-3)^2}} < \epsilon $

            \begin{itemize}
                \item $\abs*{x} \leq \norm*{(x,y-3)} < \delta$
                \item $\abs*{y-3} \leq \norm*{(x,y-3)} < \delta$
            \end{itemize}

            $\abs*{\frac{x^2(y-3)^2e^x}{x^2+(y-3)^2}} = $

            $\frac{\abs*{x^2(y-3)^2e^x}}{x^2+(y-3)^2} = $

            $\frac{x^2(y-3)^2\abs*{e^x}}{x^2+(y-3)^2} \stackrel{x\to0\Rightarrow e^x \to 1}{=} $

            $\frac{x^2(y-3)^2}{x^2+(y-3)^2} \leq$
            
            $\frac{\cancel{\norm*{(x,y-3)}^2}\norm*{(x,y-3)}^2}{\cancel{\norm*{(x,y-3)}^2}} \stackrel{\delta < 1}{\leq}$

            $ \delta = \epsilon \Rightarrow$

            $ \delta = \min(1, \epsilon) \qquad \blacksquare$

    \end{enumerate}

\end{document} 
