\documentclass[../parcial.tex]{subfiles}

\begin{document}

    \begin{enumerate}
        \item $ \int \int_D e^xy^3 dA $
        
            $D=$ \begin{itemize}
                \item $ x= y^4$
                \item $ x= 1$
            \end{itemize} $\Rightarrow$

            \begin{itemize}
                \item $ 0 \leq x \leq y^4 $
                \item $ 0 \leq y \leq 1 $
            \end{itemize}

            $ \int_0^1 (\int_0^{y^4} e^xy^3 dx) dy $

            \begin{itemize}
                \item $\int_0^{y^4} e^xy^3 dx = $
                
                    $ e^{y^4}y^3 - y^3 $
                
                \item $\int_0^1 e^{y^4}y^3 - y^3 dy = $
                
                    \qquad $\int e^{y^4}y^3 dy $

                    \qquad $ u = y^4 \wedge du = 4y^3 dy \Rightarrow dy = \frac{du}{4y^3} \Rightarrow $

                    \qquad $ \int \frac{e^u}{4} du = \frac{1}{4}e^u + C = \frac{e^{y^4}}{4} + C \Rightarrow$

                    $\int_0^1 e^{y^4}y^3 - y^3 dy \stackrel{Barrow}{=} $

                    $ \left. \frac{e^{y^4}}{4} - \frac{y^4}{4} \right |_0^1 = $

                    $ \frac{e}{4} - \frac{1}{4} - \frac{1}{4} = \frac{e-2}{4}$

            \end{itemize}

        \item
            \begin{itemize}
                \item $ x + 2y = 2$ describe un plano
                
                    $ x = 0 \Rightarrow y = 1$

                    $ y = 0 \Rightarrow x = 2$

                    Como se encuentra en el primer octante

                    $D^{\prime} = $\begin{itemize}
                        \item $0 \leq x \leq 2 - 2y$
                        \item $0 \leq y \leq 1 $
                    \end{itemize}

                \item $ z = x^2 + y^2 $ describe un paraboloide
                
                    $0 \leq z \leq x^2 + y^2$

            \end{itemize}

            $ $

            $\int_0^1( \int_0^{2-2y} (\int_0^{x^2+y^2} 1 dz) dx)dy $

            \begin{itemize}
                \item $\int_0^{x^2+y^2} 1 dz = x^2+y^2 $

                \item $ \int_0^{2-2y} x^2+y^2 dx \stackrel{Barrow}{=} $

                    $\left. \frac{x^3}{3} + xy^2 \right |_0^{2-2y} = $

                    $ y^2\left(-2y+2\right)+\frac{\left(-2y+2\right)^3}{3} $

                \item $ \int_0^1  y^2\left(-2y+2\right) + \frac{\left(-2y+2\right)^3}{3} dy = $

                    \begin{itemize}
                        \item $\int_0^1 y^2(-2y+2) dy = $

                            $ \int_0^1 -2y^3 + 2y^2 dy \stackrel{Barrow}{=} $

                            $ \left. -\frac{y^4}{2} + \frac{2y^3}{3} \right |_0^1 = $

                            $ -\frac{1}{2} + \frac{2}{3} = \frac{1}{6} $

                        \item $ \int_0^1 \frac{\left(-2y+2\right)^3}{3} dy = $
                        
                            $ \frac{1}{3} \int_0^1 -8y^3 + 24y^2 - 24y + 8 dy \stackrel{Barrow}{=} $

                            $ \frac{1}{3} ( \left. -2y^4 + 8y^3 - 12y^2 + 8y  \right |_0^1 ) = $

                            $ \frac{1}{3} ( -2 + 8 - 12 + 8 ) = \frac{2}{3}$
                    \end{itemize}

                    $ \int_0^1  y^2\left(-2y+2\right) + \frac{\left(-2y+2\right)^3}{3} dy = $
                    $\frac{1}{6} + \frac{2}{3} = \frac{5}{6}$

            \end{itemize}

    \end{enumerate}

\end{document} 
