\documentclass[../practica_01.tex]{subfiles}

\begin{document}

    \begin{enumerate}

        \item $u = (3,-4), v=(5,0)$

            $ P_{u}(v) = \frac{u \cdot v}{\norm*{u}^2}\cdot u = $
            $ \frac{(3,-4) \cdot (5,0)}{\norm*{(3,-4)}^2}\cdot (3,-4) =$

            $\frac{15}{25} \cdot (3,-4) = (\frac{9}{5},-\frac{12}{5})$

        \item $u = (1,2), v=(-4,1)$

            $ P_{u}(v) = \frac{u \cdot v}{\norm*{u}^2}\cdot u = $
            $ \frac{(1,2) \cdot (-4,1)}{\norm*{(1,2)}^2}\cdot (1,2) =$

            $-\frac{2}{5} \cdot (1,2) = (-\frac{2}{5},-\frac{4}{5})$

        \item $u = (3,6,2), v=(1,2,3)$

            $ P_{u}(v) = \frac{u \cdot v}{\norm*{u}^2}\cdot u = $
            $ \frac{(3,6,2) \cdot (1,2,3)}{\norm*{(3,6,2)}^2}\cdot (3,6,2) =$

            $\frac{3}{7} \cdot (3,6,2) = (\frac{9}{7},\frac{18}{7},\frac{6}{7})$

    \end{enumerate}

\end{document}