\documentclass[../parcial.tex]{subfiles}

\begin{document}

    \begin{enumerate}
        \item $ \lim_{(x,y) \to (1,0)} f(x,y) $

            $f(x,y) = \frac{(x-1)^2y}{(x-1)^3+y3}$

        \subsection*{Pruebo por rectas}

        \begin{itemize}
            \item recta $x = 1$
            
                $\lim_{y\to0} \frac{0}{y3} = 0 $

            \item recta $y = (x-1)$
            
                $\lim_{x\to1} \frac{\cancel{(x-1)^3}}{2\cancel{(x-1)^3}} = \frac{1}{2}$

        \end{itemize}

        Al dar distinto los limites se demuestra que $\nexists \lim_{(x,y)\to(1,0)} f(x,y) $

        \item $ \lim_{(x,y) \to (0,0)} f(x,y) $
        
            $f(x,y) = \frac{x\sin(y^2)}{x^2+y^2}$

            \subsection*{Pruebo por curvas}

            \begin{itemize}
                \item iterado $ x = 0$

                    $\lim_{y\to0} f(0,y) = $

                    $\lim_{y\to0} \frac{0}{y^2} = 0$

            \end{itemize}

            \subsection*{Intento demostrar por sandwich}
        
            $ \exists g(x,y): \lim_{(x,y)\to(0,0)} g(x,y) = 0 \wedge 0 \leq \abs*{f(x,y)} \leq \abs*{g(x,y)} $

            $ \abs*{\frac{x\sin(y^2)}{x^2+y^2}} = $

            $ \frac{\abs*{x}\abs*{\sin(y^2)}}{x^2+y^2} = $

            $ \frac{\abs*{x}\abs*{\sin(y^2)}}{x^2+y^2} \stackrel{\abs*{\sin(k)} \leq \abs*{k}}{\leq} $

            $ \frac{\abs*{x}y^2}{x^2+y^2} = $

            $ \abs*{x}\cdot\frac{y^2}{x^2+y^2} $
            
            \qquad $ x^2 \geq 0 \Rightarrow x^2 + y^2 \geq y^2 \Rightarrow 1 \geq \frac{y^2}{x^2 + y^2} : \star $
            
            $ \abs*{x}\cdot\frac{y^2}{x^2+y^2} \stackrel{\star}{\leq}$

            $ \abs*{x}\cdot 1 \stackrel{(x,y)\to (0,0)}{\to} = 0$

            $\Rightarrow 0 \leq \abs*{f(x,y)} \leq \abs*{x} $

            $ \Rightarrow $ por sandwich $\lim_{(x,y) \to (0,0)} f(x,y) = 0$

    \end{enumerate}

\end{document} 
