\documentclass[../parcial.tex]{subfiles}

\begin{document}

    \begin{enumerate}
        \item $ a = 1 \Rightarrow \lim_{(x,y) \to (0,0)} f(x,y) $

        $ f(x,y) = \frac{xy}{x^2+y^2} $

        \subsection*{Pruebo por curvas}

        \begin{itemize}
            \item iterado $x = 0$

                $\lim_{y\to0} f(0,y) = \lim_{y\to0} \frac{0y}{y^2} = 0$

            \item iterado $y = 0$

                $\lim_{x\to0} f(x,0) = \lim_{x\to0} \frac{x0}{x^2} = 0$

            \item rectas $y = mx$
            
                $\lim_{x\to0} f(x,mx) = \lim_{x\to0} \frac{m\cancel{x^2}}{\cancel{x^2}(1+m^2)} = \frac{m}{1+m^2} \wedge m \neq 0 \Rightarrow$

                $\lim_{x\to0} f(x,mx) \neq 0$

        \end{itemize}

        $ \Rightarrow $ por rectas el limite da distinto que por los iterados $ \Rightarrow \nexists \lim_{(x,y) \to (0,0)} f(x,y)$

        \item $ a = 2 \Rightarrow \lim_{(x,y) \to (0,0)} f(x,y) $
        
            $ f(x,y) = \frac{xy^2}{x^2+y^2} $
        
            \subsection*{Pruebo por curvas}

            \begin{itemize}
                \item iterado $ x = 0$

                    $\lim_{y\to0} f(0,y) = \lim_{y\to0} \frac{0y^2}{y^2} = 0$

                \item iterado $ y = 0$

                    $\lim_{x\to0} f(x,0) = \lim_{x\to0} \frac{x0}{x^2} = 0$

                \item rectas $ y = mx$
                
                    $\lim_{x\to0} f(x,mx) = \lim_{x\to0} \frac{x^3m^2}{x^2+(mx)^2} = $

                    $ \lim_{x\to0} \frac{x^3m^2}{x^2(1+m^2)} = $

                    $ \lim_{x\to0} \frac{x^{\cancel{3}}m^2}{\cancel{x^2}(1+m^2)} = 0 $

            \end{itemize}

            Estimo que $\lim_{(x,y) \to (0,0)} f(x,y) = 0$

            \subsection*{Intento demostrar por sandwich}
        
            $ \exists g(x,y): \lim_{(x,y)\to(0,0)} g(x,y) = 0 \wedge 0 \leq \abs*{f(x,y)} \leq \abs*{g(x,y)} $

            $ $

            $ \abs*{\frac{xy^2}{x^2+y^2}} = $

            $ \frac{\abs*{x}y^2}{x^2+y^2} = $

            $ \abs*{x}\frac{y^2}{x^2+y^2} = $

            $ \qquad x^2 \geq 0 \Rightarrow x^2 + y^2 \geq y^2 \Rightarrow 1 \geq \frac{y^2}{x^2+y^2} : \star $

            $ \abs*{x}\frac{y^2}{x^2+y^2} \stackrel{\star}{\leq} $

            $ \abs*{x} \cdot 1 \stackrel{(x,y)\to(0,0)}{\to} 0$

            $ \Rightarrow g(x,y) = \abs*{x} $

            $ \Rightarrow $ por sandwitch $f(x,y) \stackrel{(x,y)\to(0,0)}{\to} 0 \qquad \square$

        \item $a > 2 \Rightarrow \lim_{(x,y) \to (0,0)} f(x,y)$

            $ a = 2 + k : k > 0$

            $ f(x,y) = \frac{xy^{2+k}}{x^2+y^2} $

            Estimo que $\lim_{(x,y) \to (0,0)} f(x,y) = 0$

            \subsection*{Intento demostrar por sandwich}
        
            $ \exists g(x,y): \lim_{(x,y)\to(0,0)} g(x,y) = 0 \wedge 0 \leq \abs*{f(x,y)} \leq \abs*{g(x,y)} $

            $ $

            $ \abs*{\frac{xy^{2+k}}{x^2+y^2}} = $

            $ \frac{\abs*{x}\abs*{y^k}y^2}{x^2+y^2} = $

            $ \abs*{x}\abs*{y^k}\frac{y^2}{x^2+y^2} = $

            $ \qquad x^2 \geq 0 \Rightarrow x^2 + y^2 \geq y^2 \Rightarrow 1 \geq \frac{y^2}{x^2+y^2} : \star $

            $ \abs*{x}\abs*{y^k}\frac{y^2}{x^2+y^2} \stackrel{\star}{\leq} $

            $ \abs*{x}\abs*{y^k} \cdot 1 \stackrel{(x,y)\to(0,0)}{\to} 0\ \forall k$

            $ \Rightarrow g(x,y) = \abs*{x}\abs*{y^k}$

            $ \Rightarrow $ por sandwitch $f(x,y) \stackrel{(x,y)\to(0,0)}{\to} 0 \qquad \square$

    \end{enumerate}

    $ \Rightarrow \exists \lim_{(x,y)\to(0,0)} f(x,y) = \frac{xy^a}{x^2+y^2} \wedge \lim_{(x,y)\to(0,0)} f(x,y) = \frac{xy^a}{x^2+y^2} = 0\ \forall a \geq 2 \qquad\square$

\end{document} 
